Factorize combinators on definitions/lists to AstUtils

template-coq/theories/AstUtils.v
@@ -2,6 +2,7 @@ From Coq Require Import Ascii String Bool OrderedType.
 From Coq Require Import List.
 From Template Require Import Ast utils.
 Import List.ListNotations.
+Require Import FunctionalExtensionality.
 
 Definition map_decl f (d : context_decl) :=
   {| decl_name := d.(decl_name);
@@ -29,6 +30,20 @@ Proof.
   destruct i, i0.
   decide equality; eauto with eq_dec.
 Defined.
+
+Definition ident_eq (x y : ident) :=
+  match string_compare x y with
+  | Eq => true
+  | _ => false
+  end.
+
+Lemma ident_eq_spec x y : reflect (x = y) (ident_eq x y).
+Proof.
+  unfold ident_eq. destruct (string_compare_eq x y).
+  destruct string_compare; constructor; auto.
+  intro Heq; specialize (H0 Heq). discriminate.
+  intro Heq; specialize (H0 Heq). discriminate.
+Qed.
 
 Definition decompose_app (t : term) :=
   match t with
@@ -100,3 +115,199 @@ Proof.
     refine (List.map (fun x => remove_arity decl.(ind_npars)
                                                 (snd (fst x))) ind_ctors).
 Defined.
+
+(** Combinators *)
+
+Arguments dname {term} _.
+Arguments dtype {term} _.
+Arguments dbody {term} _.
+Arguments rarg {term} _.
+
+Definition on_snd {A B C} (f : B -> C) (p : A * B) :=
+  (fst p, f (snd p)).
+
+Definition map_def {A B : Set} (f : A -> B) (d : def A) :=
+  {| dname := d.(dname); dtype := f d.(dtype); dbody := f d.(dbody); rarg := d.(rarg) |}.
+
+Definition test_snd {A B} (f : B -> bool) (p : A * B) :=
+  f (snd p).
+
+Definition test_def {A : Set} (f : A -> bool) (d : def A) :=
+  f d.(dtype) && f d.(dbody).
+
+Definition tCaseBrsProp {A} (P : A -> Prop) (l : list (nat * A)) :=
+  Forall (fun x => P (snd x)) l.
+
+Definition tFixProp {A : Set} (P : A -> Prop) (m : mfixpoint A) :=
+  Forall (fun x : def A => P x.(dtype) /\ P x.(dbody)) m.
+
+Lemma on_snd_on_snd {A B C D} (f : C -> D) (g : B -> C) (d : A * B) :
+  on_snd f (on_snd g d) = on_snd (fun x => f (g x)) d.
+Proof.
+  destruct d; reflexivity.
+Qed.
+
+Lemma compose_on_snd {A B C D} (f : C -> D) (g : B -> C) :
+  compose (A:=A * B) (on_snd f) (on_snd g) = on_snd (compose f g).
+Proof.
+  reflexivity.
+Qed.
+
+Lemma map_def_map_def {A B C : Set} (f : B -> C) (g : A -> B) (d : def A) :
+  map_def f (map_def g d) = map_def (fun x => f (g x)) d.
+Proof.
+  destruct d; reflexivity.
+Qed.
+
+Lemma compose_map_def {A B C : Set} (f : B -> C) (g : A -> B) :
+  compose (A:=def A) (map_def f) (map_def g) = map_def (compose f g).
+Proof. reflexivity. Qed.
+
+Lemma combine_map_id {A B} (l : list (A * B)) :
+ l = combine (map fst l) (map snd l).
+Proof.
+  induction l ; simpl; try easy.
+  destruct a. now f_equal.
+Qed.
+
+Lemma map_map_compose :
+  forall (A B C : Type) (f : A -> B) (g : B -> C) (l : list A),
+    map g (map f l) = map (compose g f) l.
+Proof. apply map_map. Qed.
+Hint Unfold compose : terms.
+
+Lemma map_id_f {A} (l : list A) (f : A -> A) :
+  (forall x, f x = x) ->
+  map f l = l.
+Proof.
+  induction l; intros; simpl; try easy.
+  rewrite H. f_equal. eauto.
+Qed.
+
+Lemma map_def_id {t : Set} : map_def (@id t) = id.
+Proof. extensionality p. now destruct p. Qed.
+Hint Rewrite @map_def_id @map_id.
+
+Lemma forall_map_spec {A B} {P : A -> Prop} {l} {f g : A -> B} :
+  Forall P l -> (forall x, P x -> f x = g x) ->
+  map f l = map g l.
+Proof.
+  induction 1; simpl; trivial.
+  intros Heq. rewrite Heq. f_equal. apply IHForall. apply Heq. apply H.
+Qed.
+
+Lemma on_snd_spec {A B C} (P : B -> Prop) (f g : B -> C) (x : A * B) :
+  P (snd x) -> (forall x, P x -> f x = g x) ->
+  on_snd f x = on_snd g x.
+Proof.
+  intros. destruct x. unfold on_snd. simpl.
+  now rewrite H0; auto.
+Qed.
+
+Lemma map_def_spec {A B : Set} (P : A -> Prop) (f g : A -> B) (x : def A) :
+  P x.(dbody) -> P x.(dtype) -> (forall x, P x -> f x = g x) ->
+  map_def f x = map_def g x.
+Proof.
+  intros. destruct x. unfold map_def. simpl.
+  rewrite !H1; auto.
+Qed.
+
+Lemma case_brs_map_spec {A B : Set} {P : A -> Prop} {l} {f g : A -> B} :
+  tCaseBrsProp P l -> (forall x, P x -> f x = g x) ->
+  map (on_snd f) l = map (on_snd g) l.
+Proof.
+  intros.
+  eapply (forall_map_spec H).
+  intros.
+  eapply on_snd_spec; eauto.
+Qed.
+
+Lemma tfix_map_spec {A B : Set} {P : A -> Prop} {l} {f g : A -> B} :
+  tFixProp P l -> (forall x, P x -> f x = g x) ->
+  map (map_def f) l = map (map_def g) l.
+Proof.
+  intros.
+  eapply (forall_map_spec H).
+  intros. destruct H1;
+  eapply map_def_spec; eauto.
+Qed.
+
+Lemma forall_forallb_map_spec {A B : Type} {P : A -> Prop} {p : A -> bool}
+      {l : list A} {f g : A -> B} :
+    Forall P l -> forallb p l = true ->
+    (forall x : A, P x -> p x = true -> f x = g x) -> map f l = map g l.
+Proof.
+  induction 1; simpl; trivial.
+  rewrite andb_true_iff. intros [px pl] Hx.
+  f_equal. now apply Hx. now apply IHForall.
+Qed.
+
+Lemma on_snd_test_spec {A B C} (P : B -> Prop) (p : B -> bool) (f g : B -> C) (x : A * B) :
+  P (snd x) -> (forall x, P x -> p x = true -> f x = g x) ->
+  test_snd p x = true ->
+  on_snd f x = on_snd g x.
+Proof.
+  intros. destruct x. unfold on_snd. simpl.
+  now rewrite H0; auto.
+Qed.
+
+Lemma map_def_test_spec {A B : Set} (P : A -> Prop) p (f g : A -> B) (x : def A) :
+  P x.(dbody) -> P x.(dtype) -> (forall x, P x -> p x = true -> f x = g x) ->
+  test_def p x = true ->
+  map_def f x = map_def g x.
+Proof.
+  intros. destruct x. unfold map_def. simpl.
+  unfold test_def in H2; simpl in H2. rewrite andb_true_iff in H2.
+  rewrite !H1; intuition auto.
+Qed.
+
+Lemma case_brs_forallb_map_spec {A B : Set} {P : A -> Prop} {p : A -> bool}
+      {l} {f g : A -> B} :
+  tCaseBrsProp P l ->
+  forallb (test_snd p) l = true ->
+  (forall x, P x -> p x = true -> f x = g x) ->
+  map (on_snd f) l = map (on_snd g) l.
+Proof.
+  intros.
+  eapply (forall_forallb_map_spec H H0).
+  intros.
+  eapply on_snd_test_spec; eauto.
+Qed.
+
+Lemma tfix_forallb_map_spec {A B : Set} {P : A -> Prop} {p} {l} {f g : A -> B} :
+  tFixProp P l ->
+  forallb (test_def p) l = true ->
+  (forall x, P x -> p x = true -> f x = g x) ->
+  map (map_def f) l = map (map_def g) l.
+Proof.
+  intros.
+  eapply (forall_forallb_map_spec H H0).
+  intros. destruct H2.
+  eapply map_def_test_spec; eauto.
+Qed.
+
+Ltac apply_spec :=
+  match goal with
+  | H : Forall _ _, H' : forallb _ _ = _ |- map _ _ = map _ _ =>
+    eapply (forall_forallb_map_spec H H')
+  | H : Forall _ _ |- map _ _ = map _ _ =>
+    eapply (forall_map_spec H)
+  | H : tCaseBrsProp _ _, H' : forallb _ _ = _ |- map _ _ = map _ _ =>
+    eapply (case_brs_forallb_map_spec H H')
+  | H : tCaseBrsProp _ _ |- map _ _ = map _ _ =>
+    eapply (case_brs_map_spec H)
+  | H : tFixProp _ _, H' : forallb _ _ = _ |- map _ _ = map _ _ =>
+    eapply (tfix_forallb_map_spec H H')
+  | H : tFixProp _ _ |- map _ _ = map _ _ =>
+    eapply (tfix_map_spec H)
+  end.
+
+Lemma Forall_map {A B} (P : B -> Prop) (f : A -> B) l : Forall (Program.Basics.compose P f) l -> Forall P (map f l).
+Proof.
+  induction 1; constructor; auto.
+Qed.
+
+Lemma Forall_impl {A} (P Q : A -> Prop) : forall l, Forall P l -> (forall x, P x -> Q x) -> Forall Q l.
+Proof.
+  induction 1; constructor; auto.
+Qed.
